Finished both Sinz proofs

src/cardinality/sinz_amk.lean
@@ -5,17 +5,13 @@ Authors: Cayden Codel, Jeremy Avigad, Marijn Heule
 Carnegie Mellon University
 -/
 
-import cnf.literal
-import cnf.clause
-import cnf.cnf
-import cnf.encoding
-import cnf.gensym
-
-import cardinality.distinct
-import cardinality.cardinality
-
 import data.list.basic
-import data.nat.basic
+import cnf.cnf
+import cnf.gensym
+import cnf.encoding
+import cardinality.distinct
+import cardinality.amk
+import cardinality.alk
 
 variables {V : Type*} [inhabited V] [decidable_eq V]
 
@@ -23,74 +19,555 @@ namespace sinz_amk
 
 open list
 open literal
-open clause
 open cnf
+open clause
 open assignment
-open encoding
---open distinct
+open distinct
+open prod
 open gensym
---open amo
+open encoding
+open amk
+open alk
+open nat
 
-variables {l : list (literal V)} {lit l₁ l₂ : literal V} {g : gensym V}
-          {τ : assignment V} (hdis : disjoint g.stock (clause.vars l))
-          {c : clause V}
-          {k : nat} (hk : k ≥ 2)
+def S (g : gensym V) (l : list (literal V)) (r c : nat) : V := 
+  g.nth ((r * length l) + c)
 
--- Not true, refine later
-lemma a1 {k : nat} : k ≥ 2 → ∀ m, m < k :=
+theorem S_not_mem_vars {g : gensym V} {l : list (literal V)} 
+  (hdis : disjoint g.stock (clause.vars l)) : 
+  ∀ (r c : nat), S g l r c ∉ clause.vars l :=
 begin
-  sorry
+  intros r c,
+  rw S,
+  have h₁ := set.disjoint_left.mp hdis,
+  have h₂ := (nth_mem_stock g (r * length l + c)),
+  exact h₁ h₂
 end
 
-lemma a2 {k : nat} {l : list V} : k ≥ 2 → length l = k → length l ≥ 2 :=
+def signal_row_prop (k : nat) (g : gensym V) (l : list (literal V)) (r c : nat) : cnf V :=
+  ite (r < k + 1 ∧ c < length l - 1) 
+  [[Neg (S g l r c), Pos (S g l r (c + 1))]] []
+
+def first_prop (g : gensym V) (l : list (literal V)) (r c : nat) : cnf V :=
+  if hidx : (r = 0 ∧ c < length l) then
+    [[(l.nth_le c hidx.2).flip, Pos (S g l 0 c)]] 
+  else []
+
+def inc_prop (k : nat) (g : gensym V) (l : list (literal V)) (r c : nat) : cnf V :=
+  if hidx : (r < k ∧ c < length l - 1 ∧ c + 1 < length l) then
+    [[(l.nth_le (c + 1) hidx.2.2).flip, Neg (S g l r c), Pos (S g l (r + 1) (c + 1))]]
+  else []
+
+def sinz_amk (k : nat) (g : gensym V) (l : list (literal V)) : cnf V :=
+if k ≤ 1 ∨ length l ≤ k then [] else
+join ((range (k + 1)).map (λ i, join
+    ((range (length l)).map (λ j,
+      signal_row_prop k g l i j ++
+      first_prop g l i j ++
+      inc_prop k g l i j))
+  )) ++ [[Neg (S g l k (length l - 1))]]
+
+lemma helper {k c n : nat} : 1 < k → k < n → c < n - 1 → c < n :=
 begin
-  sorry
+  intros hk hn hc,
+  rcases exists_eq_add_of_lt (lt_trans hk hn) with ⟨m, hm⟩,
+  subst hm,
+  simp at hc,
+  exact lt_succ_of_lt hc
 end
 
-lemma disjoint_fresh_of_disjoint : disjoint g.stock (clause.vars (lit :: l)) → 
-  disjoint (g.nfresh k).2.stock (clause.vars l) :=
+theorem signal_row_prop_mem {k r c : nat} {l : list (literal V)} 
+  (hk : k > 1) (hl : length l > k) (g : gensym V) 
+  (hr : r < k + 1) (hc : c < length l - 1) :
+  [Neg (S g l r c), Pos (S g l r (c + 1))] ∈ sinz_amk k g l :=
 begin
-  sorry
+  rw sinz_amk,
+  simp [not_le.mpr hl, not_le.mpr hk],
+  use [r, hr, c, helper hk hl hc],
+  left,
+  rw signal_row_prop,
+  simp [hr, hc]
 end
 
-def sinz_k {k : nat} (hk : k ≥ 2) : Π (l : list (literal V)), Π (g : gensym V),
-  (disjoint g.stock (clause.vars l)) → cnf V
-| [] _ _ := []
-| [l₁] _ _ := [] -- [l₁.flip, Neg (g.prev)]
-| (l₁ :: l₂ :: ls) g hdis :=
-  --let ⟨ss, g'⟩ := g.nfresh k in
-  have hlen₁ : length (g.nfresh k).1 ≥ 2, from a2 hk (length_list_nfresh g k),
-  have hlen₂ : length ((g.nfresh k).2.nfresh k).1 ≥ 2, 
-    from a2 hk (length_list_nfresh (g.nfresh k).2 k),
-  -- x_i → s_(i, 1)
-  [l₁.flip, Pos (nth_le (g.nfresh k).1 0 (a1 hlen₁ _))] ::
+theorem first_prop_mem {k c : nat} {l : list (literal V)}
+  (hk : k > 1) (hl : length l > k) (g : gensym V)
+  (hc : c < length l) :
+  [(l.nth_le c hc).flip, Pos (S g l 0 c)] ∈ sinz_amk k g l :=
+begin
+  rw sinz_amk,
+  simp [not_le.mpr hl, not_le.mpr hk],
+  use 0,
+  simp,
+  use [c, hc],
+  right, left,
+  rw first_prop,
+  simp [hc]
+end
 
-  -- x_(i + 1) → ¬s_(i, k)
-  [l₂.flip, Neg (nth_le (g.nfresh k).1 (k - 1) (a1 hlen₁ _))] ::
+theorem inc_prop_mem {k r c : nat} {l : list (literal V)} 
+  (hk : k > 1) (hl : length l > k) (g : gensym V) 
+  (hr : r < k) (hc₁ : c < length l - 1) (hc₂ : c + 1 < length l) :
+  [(l.nth_le (c + 1) hc₂).flip, Neg (S g l r c), Pos (S g l (r + 1) (c + 1))] ∈ sinz_amk k g l :=
+begin
+  rw sinz_amk,
+  simp [not_le.mpr hk, not_le.mpr hl],
+  use [r, lt_succ_of_lt hr, c, lt_of_succ_lt hc₂],
+  right, right,
+  rw inc_prop,
+  simp [hr, hc₁, hc₂]
+end
 
-  -- s_(i, j) → s_(i + 1, j)
-  (map (λ p : (nat × V), let ⟨i, s⟩ := p in 
-      [Neg s,
-       Pos (nth_le ((g.nfresh k).2.nfresh k).1 i (a1 hlen₂ _))])
-    (enum (g.nfresh k).1))
-  ++
-  (map (λ p : (nat × V), let ⟨i, s⟩ := p in
-      [l₂.flip, Neg s, Pos (nth_le ((g.nfresh k).2.nfresh k).1 (i + 1) (a1 hlen₂ _))])
-      (enum (take (k - 1) (g.nfresh k).1)))
-  ++
-  sinz_k (l₂ :: ls) (g.nfresh k).2 (disjoint_fresh_of_disjoint hdis)
+-- First arg is row, second is col in (k + 1) × |l| matrix
+def signal_truth (l : list (literal V)) 
+  (g : gensym V) (τ : assignment V) : nat → nat → bool
+| 0       0       := l.head.eval τ 
+| 0       (c + 1) := if h : (c + 1) < length l then 
+                      (l.nth_le (c + 1) h).eval τ || signal_truth 0 c 
+                     else ff
+| (r + 1) 0       := ff
+| (r + 1) (c + 1) := if h : (c + 1) < length l then
+                      ((l.nth_le (c + 1) h).eval τ ∧ signal_truth r c) ||
+                       signal_truth (r + 1) c
+                     else ff
 
-def sinz {k : nat} (hk : k ≥ 2) : Π (l : list (literal V)), Π (g : gensym V),
-  (disjoint g.stock (clause.vars l)) → cnf V
-| l g hdis := (sinz_k hk l g hdis) ++ 
-              -- ¬s_(1, j) for j > 1
-              map (λ s, [Neg s]) (g.nfresh k).1.tail
+def rc_from_var (l : list (literal V)) (g : gensym V) (v : V) : nat → nat → (nat × nat)
+| 0       0       := ⟨0, 0⟩
+| 0       (c + 1) := if v = g.nth (c + 1) then ⟨0, c + 1⟩ else rc_from_var 0 c
+| (r + 1) 0       := if v = g.nth ((r + 1) * length l) then ⟨r + 1, 0⟩ 
+                     else rc_from_var r (length l - 1)
+| (r + 1) (c + 1) := if v = g.nth ((r + 1) * length l + c + 1) then ⟨r + 1, c + 1⟩
+                     else rc_from_var (r + 1) c
 
-/-
-    [l₁.flip, Pos (g.fresh.1)] :: 
-    [Neg g.fresh.1, Pos g.fresh.2.fresh.1] ::
-    [Neg g.fresh.1, l₂.flip] ::
-    (sinz (l₂ :: ls) g.fresh.2 (disjoint_fresh_of_disjoint hdis))
--/
+def sinz_tau (k : nat) (l : list (literal V))
+  (g : gensym V) (τ : assignment V) : assignment V :=
+  λ v, if v ∈ clause.vars l then τ v else
+         signal_truth l g τ (rc_from_var l g v k (length l - 1)).1 (rc_from_var l g v k (length l - 1)).2
+
+lemma help {a b c : nat} : b ≤ c → a + b ≤ a + c :=
+begin
+  exact (add_le_add_iff_left a).mpr
+end
+
+theorem rc_helper {r r' c c' : nat} (g : gensym V) {l : list (literal V)} :
+  r ≤ r' → c < length l → c' < length l → 
+  (r = r' → c ≤ c') → 
+  rc_from_var l g (S g l r c) r' c' = ⟨r, c⟩ :=
+begin
+  intros hr hc hc' hreq,
+  have hrc : (r * length l + c) ≤ (r' * length l + c'),
+  { rcases eq_or_lt_of_le hr with ⟨rfl | hr⟩,
+    { exact add_le_add_left (hreq h) _ },
+    { rcases exists_eq_add_of_lt h with ⟨m, hm⟩,
+      simp [hm, add_mul, add_assoc],
+      rw [add_comm, add_assoc],
+      exact le_add_right (le_of_lt hc) } },
+  induction r' with r' ihr generalizing c',
+  { simp at hr,
+    subst hr,
+    induction c' with c' ihc; simp at hrc,
+    { subst hrc,
+      simp [rc_from_var] },
+    { rcases eq_or_lt_of_le hrc with (rfl | hrc),
+      { simp [rc_from_var, S] },
+      { simp at ihc,
+        rw ← ihc (lt_of_succ_lt hc') (le_of_lt_succ hrc) (le_of_lt_succ hrc),
+        have : c ≠ c' + 1, from ne_of_lt hrc,
+        simp [rc_from_var, S, nth_ne_of_ne this] } } },
+  { rcases eq_or_lt_of_le hr with (rfl | hr),
+    { induction c' with c' ihc;
+      simp at hrc,
+      { simp [rc_from_var, hrc, S] },
+      { have ihred := ihc (lt_of_succ_lt hc'),
+        simp at ihred,
+        rcases eq_or_lt_of_le hrc with (rfl | hrc),
+        { simp [rc_from_var, S, add_assoc] },
+        { rw ← ihred (le_of_lt_succ hrc),
+          have : (r' + 1) * l.length + c ≠ (r' + 1) * l.length + c' + 1,
+          { intro heq,
+            rw add_assoc at heq,
+            have := add_left_cancel heq,
+            rw this at hrc,
+            exact nat.lt_asymm hrc hrc },
+          simp [rc_from_var, S, nth_ne_of_ne this], exact le_of_lt_succ hrc } } },
+    { have hlen : length l - 1 < length l,
+      { cases l with l₁ ls,
+        { simp at hc', contradiction },
+        { simp } },
+      have : c ≤ length l - 1,
+      { cases l with l₁ ls,
+        { simp at hc, contradiction },
+        { simp at hc |-, exact le_of_lt_succ hc } },
+      have ihred := ihr (le_of_lt_succ hr) hlen (imp_intro this),
+      induction c' with c' ihc,
+      { have : r * l.length + c ≠ (r' + 1) * l.length,
+        { rcases exists_eq_add_of_lt hr with ⟨m, hm⟩,
+          intro heq,
+          simp [← succ_eq_add_one, hm] at heq,
+          rw [succ_mul, add_mul, add_assoc] at heq,
+          have heqc := add_left_cancel_iff.mp heq,
+          have : l.length ≤ m * l.length + l.length, from le_add_self,
+          have := lt_of_lt_of_le hc this,
+          exact absurd heqc (ne_of_lt this) },
+        simp [rc_from_var, S, nth_ne_of_ne this],
+        rw ← S,
+        apply ihred,
+        have h₁ : r * l.length ≤ r' * l.length,
+        { exact nat.mul_le_mul_right _ (le_of_lt_succ hr) },
+        have h₂ : c ≤ l.length - 1,
+        { cases l with l₁ ls,
+          { simp at hc, contradiction },
+          { simp at hc, exact le_of_lt_succ hc } },
+        exact add_le_add h₁ h₂, },
+      { have : r * l.length + c ≤ (r' + 1) * l.length + c',
+        { rw [add_mul, add_assoc],
+          apply add_le_add,
+          { exact nat.mul_le_mul_right _ (le_of_lt_succ hr) },
+          { rw one_mul,
+            exact le_add_right (le_of_lt hc) } },
+        have himp : r = r' + 1 → c ≤ c',
+        { rintro rfl,
+          exact (add_le_add_iff_left ((r' + 1) * l.length)).mp this },
+        rw ← ihc (lt_of_succ_lt hc') himp,
+        have : r * l.length + c ≠ (r' + 1) * l.length + c' + 1,
+        { exact ne_of_lt (lt_succ_of_le this) },
+        simp [rc_from_var, S, nth_ne_of_ne this], exact this } } }
+end
+
+theorem rc_helper' {r r' c c' : nat} (g : gensym V) {l : list (literal V)} :
+  r ≤ r' → c < length l → c' < length l → c ≤ c' →
+  rc_from_var l g (S g l r c) r' c' = ⟨r, c⟩ :=
+assume hr hc hc' hle, rc_helper g hr hc hc' (imp_intro hle)
+
+-- Forward direction --
+lemma sub_helper {n m : nat} : n < m → m - 1 < m :=
+begin
+  intro h,
+  cases m,
+  { simp at h, contradiction },
+  { simp, exact lt_succ_self m }
+end
+
+theorem signal_semantics {k r c : nat} (hk : k > 1) {l : list (literal V)} {g : gensym V}
+  (hdis : disjoint g.stock (clause.vars l))
+  (hr : r < k + 1) (hc : c < length l) :
+  ∀ {τ : assignment V}, 
+  (signal_truth l g τ r c) = tt ↔ (alk.eval (r + 1) τ (l.take (c + 1))) = tt :=
+begin
+  intro τ,
+  induction r with r ihr generalizing c,
+  { induction c with c ihc,
+    { simp [signal_truth, take_one_of_ne_nil (ne_nil_of_length_pos hc),
+        alk.eval, alk, bool_symm] },
+    { simp [signal_truth, hc],
+      split,
+      { rintros (hs | hs),
+        { rw eval_take_tail_pos hc hs,
+          exact eval_zero _ _ },
+        { have ihred := (ihc (lt_of_succ_lt hc)).mp hs,
+          have := take_sublist_of_le (le_succ (c + 1)) l,
+          exact eval_tt_of_sublist_of_eval_tt this ihred } },
+      { intro hl,
+        cases h : (l.nth_le (c + 1) _).eval τ,
+        { rw eval_take_tail_neg hc h at hl,
+          exact or.inr ((ihc (lt_of_succ_lt hc)).mpr hl) },
+        { simp only [eq_self_iff_true, true_or] } } } },
+  {
+    induction c with c ihc,
+    { simp [signal_truth, take_one_of_ne_nil (ne_nil_of_length_pos hc),
+        alk.eval, alk, bool_symm],
+      cases h : literal.eval τ l.head; { simp } },
+    {
+      simp [signal_truth, hc],
+      split,
+      { rintros (⟨hs₁, hs₂⟩ | hs),
+        { rw eval_take_tail_pos hc hs₁,
+          exact (ihr (lt_of_succ_lt hr) (lt_of_succ_lt hc)).mp hs₂ },
+        { have ihred := (ihc (lt_of_succ_lt hc)).mp hs,
+          have : take (c + 1) l <+ take (c + 1 + 1) l,
+          { exact take_sublist_of_le (le_succ (c + 1)) _ },
+          exact eval_tt_of_sublist_of_eval_tt this ihred } },
+      { intro hl,
+        cases h : (l.nth_le (c + 1) _).eval τ,
+        { rw eval_take_tail_neg hc h at hl,
+          exact or.inr ((ihc (lt_of_succ_lt hc)).mpr hl) },
+        { rw eval_take_tail_pos hc h at hl,
+          exact or.inl ⟨rfl, (ihr (lt_of_succ_lt hr) (lt_of_succ_lt hc)).mpr hl⟩ } } } }
+end
+
+theorem sr_eval_tt_st {k r c : nat} (hk : k > 1) {l : list (literal V)} {g : gensym V}
+  (hdis : disjoint g.stock (clause.vars l))
+  (hr : r < k + 1) (hc : c < length l - 1) :
+  ∀ (τ : assignment V), (signal_row_prop k g l r c).eval (sinz_tau k l g τ) = tt :=
+begin
+  intro τ,
+  rw eval_tt_iff_forall_clause_eval_tt,
+  intros cl hcl,
+  simp [signal_row_prop, hr, hc] at hcl,
+  subst hcl,
+  rw eval_tt_iff_exists_literal_eval_tt,
+  cases hs : (sinz_tau k l g τ) (S g l r c),
+  { use Neg (S g l r c), simp [literal.eval, hs] },
+  { use Pos (S g l r (c + 1)),
+    have hc' : c + 1 < length l,
+    { cases l with l₁ ls,
+      { simp at hc, contradiction },
+      { cases ls with l₂ ls,
+        { simp at hc, contradiction },
+        { simp at hc, simp [hc] } } },
+    have hc'' : c < length l, from lt_of_succ_lt hc',
+    have hc''' : c + 1 ≤ length l - 1,
+    { cases l with l₁ ls,
+      { simp at hc'', contradiction },
+      { simp at hc' |-, exact succ_le_of_lt hc' } },
+    simp [literal.eval, sinz_tau, S_not_mem_vars hdis,
+      rc_helper g (le_of_lt_succ hr) hc' (sub_helper hc'') (imp_intro hc''')],
+    simp [sinz_tau, S_not_mem_vars hdis] at hs,
+    rw rc_helper g (le_of_lt_succ hr) hc'' (sub_helper hc'') 
+      (imp_intro (le_of_succ_le hc''')) at hs,
+    simp at hs,
+    cases r; { simp [signal_truth, hc'], exact or.inr hs } }
+end
+
+theorem fp_eval_tt_st {k r c : nat} (hk : k > 1) {l : list (literal V)} {g : gensym V}
+  (hdis : disjoint g.stock (clause.vars l))
+  (hr : r < k + 1) (hc : c < length l) :
+  ∀ (τ : assignment V), (first_prop g l r c).eval (sinz_tau k l g τ) = tt :=
+begin
+  intro τ,
+  rw eval_tt_iff_forall_clause_eval_tt,
+  intros cl hcl,
+  cases r,
+  { simp [first_prop, hc] at hcl,
+    subst hcl,
+    rw eval_tt_iff_exists_literal_eval_tt,
+    cases hl : (l.nth_le c hc).eval τ,
+    { use (l.nth_le c hc).flip,
+      have hmem := mem_vars_of_mem (nth_le_mem l c hc),
+      cases l.nth_le c hc;
+      { rw var at hmem,
+        rw literal.eval at hl,
+        simp [eval_flip, hl, sinz_tau, literal.eval, hmem] } },
+    { use Pos (S g l 0 c),
+      simp [literal.eval, sinz_tau, S_not_mem_vars hdis],
+      have : c ≤ length l - 1,
+      { cases l with l₁ ls,
+        { simp at hc, contradiction },
+        { simp at hc |-, exact le_of_lt_succ hc } },
+      rw rc_helper g (le_of_lt_succ hr) hc (sub_helper hc) (imp_intro this),
+      cases c,
+      { rw signal_truth,
+        rw nth_le_zero at hl,
+        exact hl },
+      { rw signal_truth,
+        simp [hc], exact or.inl hl } } },
+  { simp [first_prop, hc] at hcl, contradiction }
+end
+
+theorem ip_eval_tt_st {k r c : nat} (hk : k > 1) {l : list (literal V)} {g : gensym V}
+  (hdis : disjoint g.stock (clause.vars l))
+  (hr : r < k) (hc : c < length l - 1) :
+  ∀ (τ : assignment V), (inc_prop k g l r c).eval (sinz_tau k l g τ) = tt :=
+begin
+  intro τ,
+  rw eval_tt_iff_forall_clause_eval_tt,
+  intros cl hcl,
+  rw inc_prop at hcl,
+  have hc' : c + 1 < length l,
+  { cases l with l₁ ls,
+    { simp at hc, contradiction },
+    { cases ls with l₂ ls,
+      { simp at hc, contradiction },
+      { simp at hc, simp [hc] } } },
+  simp [hr, hc, hc'] at hcl,
+  subst hcl,
+  rw eval_tt_iff_exists_literal_eval_tt,
+  cases hs₁ : (l.nth_le _ hc').eval (sinz_tau k l g τ),
+  { use (l.nth_le _ hc').flip,
+    simp [eval_flip, hs₁] },
+  { cases hs₂ : (sinz_tau k l g τ) (S g l r c),
+    { use Neg (S g l r c), simp [literal.eval, hs₂] },
+    { use Pos (S g l (r + 1) (c + 1)),
+      have hmem := mem_vars_of_mem (nth_le_mem l _ hc'),
+      simp [literal.eval, hs₂],
+      simp [sinz_tau, S_not_mem_vars hdis] at hs₂ |-,
+      rw rc_helper g (le_of_lt hr) (lt_of_succ_lt hc') (sub_helper hc')
+         (imp_intro (le_of_lt hc)) at hs₂,
+      simp at hs₂,
+      have : c + 1 ≤ length l - 1,
+      { cases l with l₁ ls,
+        { simp at hc', contradiction },
+        { simp at hc |-, exact succ_le_of_lt hc } },
+      rw rc_helper g (succ_le_of_lt hr) hc' (sub_helper hc') (imp_intro this),
+      rw signal_truth,
+      simp [hc'],
+      cases l.nth_le _ hc';
+      { rw var at hmem,
+        simp [sinz_tau, literal.eval, hmem] at hs₁,
+        simp [literal.eval],
+        exact or.inl ⟨hs₁, hs₂⟩ } } }
+end
+
+theorem sinz_forward {k : nat} (hk : k > 1) {τ} {l : list (literal V)} {g : gensym V}
+  (hdis : disjoint g.stock (clause.vars l)) :
+  amk.eval k τ l = tt → (sinz_amk k g l).eval (sinz_tau k l g τ) = tt :=
+begin
+  intro hmk,
+  rw eval_tt_iff_forall_clause_eval_tt,
+  intros cl hcl,
+  by_cases hl : length l > k,
+  { simp [sinz_amk, not_le.mpr hk, not_le.mpr hl] at hcl,
+    rcases hcl with (⟨r, hr, c, hc, hmem⟩ | rfl),
+    { rcases hmem with (hmem | hmem | hmem),
+      { by_cases hc' : c < length l - 1,
+        { have := sr_eval_tt_st hk hdis hr hc' τ,
+          exact eval_tt_iff_forall_clause_eval_tt.mp this _ hmem },
+        { simp [signal_row_prop, hr, hc'] at hmem, contradiction } },
+      { have := fp_eval_tt_st hk hdis hr hc τ,
+        exact eval_tt_iff_forall_clause_eval_tt.mp this _ hmem },
+      { by_cases hc' : c < length l - 1,
+        { by_cases hr' : r < k,
+          { have := ip_eval_tt_st hk hdis hr' hc' τ,
+          exact eval_tt_iff_forall_clause_eval_tt.mp this _ hmem },
+          { simp [inc_prop, hr'] at hmem, contradiction } },
+        { simp [inc_prop, hc'] at hmem, contradiction } } },
+    { have : length l - 1 < length l,
+      { rcases exists_eq_add_of_lt (lt_trans hk hl) with ⟨m, hm⟩,
+        simp [hm] },
+      simp [eval_tt_iff_exists_literal_eval_tt, literal.eval,
+        sinz_tau, S_not_mem_vars hdis],
+      rw rc_helper g (le_refl k) this this (imp_intro (le_refl _)),
+      rw amk_eval_eq_alk_succ_eval at hmk,
+      simp at hmk,
+      have hmt := mt (signal_semantics hk hdis (lt_succ_self k) this).mp,
+      have : length l - 1 + 1 = length l,
+      { rcases exists_eq_add_of_lt (lt_trans hk hl) with ⟨m, hm⟩,
+        simp [hm] },
+      simp [this] at hmt,
+      exact hmt hmk } },
+  { simp [sinz_amk, not_lt.mp hl] at hcl, contradiction }
+end
+
+-- Reverse direction --
+
+theorem sr_eval_tt {τ} {k r c : nat} {g : gensym V} {l : list (literal V)}
+  (hk : k > 1) (hl : length l > k)
+  (hdis : disjoint g.stock (clause.vars l))
+  (hr : r < k + 1) (hc : c < length l - 1) :
+  (sinz_amk k g l).eval τ = tt →
+  τ (S g l r c) = tt → ∀ {c₂ : nat}, (c₂ > c ∧ c₂ < length l) → τ (S g l r c₂) = tt :=
+begin
+  rintros hs ht c₂ ⟨hgt, hcl⟩,
+  induction c₂ with c₂ ih,
+  { linarith },
+  { by_cases hcc : c = c₂,
+    { subst hcc,
+      have := signal_row_prop_mem hk hl g hr hc,
+      have := eval_tt_iff_forall_clause_eval_tt.mp hs _ this,
+      simp [eval_tt_iff_exists_literal_eval_tt] at this,
+      rcases this with ⟨lit, (rfl | rfl), hlit⟩,
+      { simp [literal.eval, ht] at hlit, contradiction },
+      { rw literal.eval at hlit, exact hlit } },
+    { have := lt_of_le_of_ne (le_of_lt_succ hgt) hcc,
+      have ihred := ih this (lt_of_succ_lt hcl),
+      have : c₂ < l.length - 1,
+      { rcases exists_eq_add_of_lt (lt_trans hk hl) with ⟨m, hm⟩,
+        simp [hm] at hcl |-,
+        exact succ_lt_succ_iff.mp hcl },
+      have := signal_row_prop_mem hk hl g hr this,
+      have := eval_tt_iff_forall_clause_eval_tt.mp hs _ this,
+      simp [eval_tt_iff_exists_literal_eval_tt] at this,
+      rcases this with ⟨lit, (rfl | rfl), hlit⟩,
+      { simp [literal.eval, ihred] at hlit, contradiction },
+      { rw [literal.eval] at hlit, exact hlit } } }
+end
+
+theorem fp_eval_tt {τ} {k r c : nat} {g : gensym V} {l : list (literal V)}
+  (hk : k > 1) (hl : length l > k)
+  (hdis : disjoint g.stock (clause.vars l))
+  (hr : r < k + 1) (hc : c < length l) :
+  (sinz_amk k g l).eval τ = tt →
+  alk.eval (r + 1) τ (l.take (c + 1)) = tt → τ (S g l r c) = tt :=
+begin
+  intros hs hlk,
+  induction c with c ih generalizing r,
+  { cases l with l ls,
+    { rw length at hc, exact absurd hc (gt_irrefl _) },
+    { simp [alk.eval, alk] at hlk,
+      cases hlit : l.eval τ,
+      { simp [hlit] at hlk, contradiction },
+      { simp [hlit] at hlk,
+        subst hlk,
+        rw eval_tt_iff_forall_clause_eval_tt at hs,
+        have := hs _ (first_prop_mem hk hl g hc),
+        simp [eval_tt_iff_exists_literal_eval_tt] at this,
+        rcases this with ⟨lit, (rfl | rfl), hlit₂⟩,
+        { rw [eval_flip, hlit] at hlit₂, contradiction },
+        { rw literal.eval at hlit₂, exact hlit₂ } } } },
+  { have hc' : c < length l - 1,
+    { rcases exists_eq_add_of_lt (lt_trans hk hl) with ⟨m, hm⟩,
+      simp [hm] at hc |-,
+      exact succ_lt_succ_iff.mp hc },
+    cases hx : literal.eval τ (l.nth_le _ hc),
+    { rw eval_take_tail_neg hc hx at hlk,
+      have ihred := ih (lt_of_succ_lt hc) hr hlk,
+      exact sr_eval_tt hk hl hdis hr hc' hs ihred ⟨lt_succ_self c, hc⟩ },
+    { rw eval_take_tail_pos hc hx at hlk,
+      rw eval_tt_iff_forall_clause_eval_tt at hs,
+      cases r,
+      { have := hs _ (first_prop_mem hk hl g hc),
+        simp [eval_tt_iff_exists_literal_eval_tt] at this,
+        rcases this with ⟨lit, (rfl | rfl), hlit⟩,
+        { simp [eval_flip, hx] at hlit, contradiction },
+        { rw literal.eval at hlit, exact hlit } },
+      { have ihred := ih (lt_of_succ_lt hc) (lt_of_succ_lt hr) hlk,
+        have := hs _ (inc_prop_mem hk hl g (succ_lt_succ_iff.mp hr) hc' hc),
+        simp [eval_tt_iff_exists_literal_eval_tt] at this,
+        rcases this with ⟨lit, (rfl | rfl | rfl), hlit⟩,
+        { rw [eval_flip, hx] at hlit, contradiction },
+        { rw [literal.eval, ihred] at hlit, contradiction },
+        { rw literal.eval at hlit, exact hlit } } } }
+end
+
+theorem sinz_reverse {k : nat} (hk : k > 1) {τ} {l : list (literal V)} {g : gensym V}
+  (hdis : disjoint g.stock (clause.vars l)) :
+  (sinz_amk k g l).eval τ = tt → amk.eval k τ l = tt :=
+begin
+  intro hs,
+  have hs_copy := hs,
+  by_cases hl : length l > k,
+  { simp [sinz_amk, not_le.mpr hk, not_le.mpr hl,   
+      eval_tt_iff_forall_clause_eval_tt] at hs,
+    have := hs _ (or.inr rfl),
+    simp [eval_tt_iff_exists_literal_eval_tt, literal.eval] at this,
+    have hl' : length l - 1 < length l,
+    { rcases exists_eq_add_of_lt (lt_trans hk hl) with ⟨m, hm⟩,
+      simp [hm] },
+    have hl'' : length l - 1 + 1 = length l,
+    { rcases exists_eq_add_of_lt (lt_trans hk hl) with ⟨m, hm⟩,
+      simp [hm] },
+    have hmt := mt (fp_eval_tt hk hl hdis (lt_succ_self k) hl' hs_copy),
+    simp at hmt,
+    have := hmt this,
+    simp [hl''] at this,
+    have hamkalk := amk_eval_eq_alk_succ_eval k τ l,
+    rw [this, bool.bnot_false] at hamkalk,
+    exact hamkalk },
+  { exact eval_tt_of_ge_length (not_lt.mp hl) _ }
+end
+
+theorem sinz_amk_encodes_amk {k : nat} (hk : k > 1) {l : list (literal V)} {g : gensym V}
+  (hdis : disjoint g.stock (clause.vars l)) :
+  encodes (amk k) (sinz_amk k g l) l :=
+begin
+  intro τ, split,
+  { intro hmk,
+    use sinz_tau k l g τ,
+    split,
+    { exact sinz_forward hk hdis hmk },
+    { intros v hv, simp [sinz_tau, hv] } },
+  { rintros ⟨σ, hs, heqod⟩,
+    rw [← amk.eval, eval_eq_amk_of_eqod _ heqod],
+    exact sinz_reverse hk hdis hs }
+end
 
 end sinz_amk
